Spec.AVL.fst
@@ -11,16 +11,16 @@ open Spec.BST
 //@AVL
 //complexity: O(n), where n is the size of the tree
 //not for effective use
-let rec is_balanced_g (#a: Type) (x: tree a)
+let rec is_balanced_global (#a: Type) (x: tree a)
   : GTot bool
   = match x with
   | Leaf -> true
   | Node data left right _ _ ->
     M.abs(height_of_tree right - height_of_tree left) <= 1 &&
-    is_balanced_g right &&
-    is_balanced_g left
+    is_balanced_global right &&
+    is_balanced_global left
 
-let is_balanced (#a: Type) (t: wdm a)
+let is_balanced_local (#a: Type) (t: wdm a)
   : bool
   = match t with
   | Leaf -> true
@@ -33,17 +33,17 @@ let is_balanced_spec_lemma (#a: Type) (t: wdm a)
   : Lemma
   (requires
     Node? t /\
-    is_balanced_g (cleft t) /\
-    is_balanced_g (cright t) /\
-    is_balanced t)
+    is_balanced_global (cleft t) /\
+    is_balanced_global (cright t) /\
+    is_balanced_local t)
   (ensures
-    is_balanced_g t
+    is_balanced_global t
   )
   = ()
 
 //@AVL
 let is_avl (#a: Type) (cmp:cmp a) (x: tree a) : GTot bool =
-  is_bst cmp x && is_balanced_g x
+  is_bst cmp x && is_balanced_global x
 
 //@AVL
 let avl (a: Type) (cmp:cmp a) = x: wdm a {is_avl cmp x}
@@ -61,7 +61,7 @@ TODO : optimize rotate_*, remove matching and add precondition
 TODO : option.get
 *)
 
-let rebalance_avl_wdm (#a: Type) (t: wdm a) : wdm a =
+let rebalance_avl (#a: Type) (t: wdm a) : wdm a =
   if Leaf? t then t else
   let Node data left right size height = t in
   if hot_wdh left - hot_wdh right > 1 then (
@@ -90,8 +90,8 @@ let rebalance_avl_wdm (#a: Type) (t: wdm a) : wdm a =
     t
   )
 
-let rebalance_avl_wds_size (#a: Type) (t: wdm a)
-  : Lemma (size_of_tree (rebalance_avl_wdm t) == size_of_tree t)
+let rebalance_avl_size (#a: Type) (t: wdm a)
+  : Lemma (size_of_tree (rebalance_avl t) == size_of_tree t)
   =
   if Leaf? t then () else
   let Node data left right size height = t in
@@ -114,25 +114,25 @@ let rebalance_avl_wds_size (#a: Type) (t: wdm a)
   )
 
 #push-options "--z3rlimit 50"
-let rebalance_avl_wds_proof (#a: Type) (cmp: cmp a) (t: wdm a)
+let rebalance_avl_proof (#a: Type) (cmp: cmp a) (t: wdm a)
   (root: a)
   : Lemma
   (requires is_bst cmp t /\ (
     match t with
     | Leaf -> True
     | Node data left right _ _ ->
-        is_balanced_g left /\
-        is_balanced_g right /\
+        is_balanced_global left /\
+        is_balanced_global right /\
         hot_wdh left - hot_wdh right <= 2 /\
         hot_wdh right - hot_wdh left <= 2
   ))
   (ensures
-    is_avl cmp (rebalance_avl_wdm t)
+    is_avl cmp (rebalance_avl t)
     /\
     (forall_keys t (key_left cmp root)
-      ==> forall_keys (rebalance_avl_wdm t) (key_left cmp root)) /\
+      ==> forall_keys (rebalance_avl t) (key_left cmp root)) /\
     (forall_keys t (key_right cmp root)
-      ==> forall_keys (rebalance_avl_wdm t) (key_right cmp root))
+      ==> forall_keys (rebalance_avl t) (key_right cmp root))
   )
   =
   if Leaf? t then () else
@@ -160,7 +160,6 @@ let rebalance_avl_wds_proof (#a: Type) (cmp: cmp a) (t: wdm a)
   ) else if hot_wdh right - hot_wdh left > 1 then (
     assert (hot_wdh right - hot_wdh left == 2);
     let Node _ rleft rright _ _ = right in
-    assert (is_balanced right);
     if hot_wdh rright >= hot_wdh rleft then (
       let r = rotate_left t in
       assert (Some? r);
@@ -183,9 +182,9 @@ let rebalance_avl_wds_proof (#a: Type) (cmp: cmp a) (t: wdm a)
 
 (** Insertion **)
 
-let rebalance_preserves_bst (#a: Type) (cmp: cmp a) (t: wdm a)
+let rebalance_avl_preserves_bst (#a: Type) (cmp: cmp a) (t: wdm a)
   : Lemma
-  (is_bst cmp t = is_bst cmp (rebalance_avl_wdm t))
+  (is_bst cmp t = is_bst cmp (rebalance_avl t))
   =
   if Leaf? t then () else
   let Node data left right size height = t in
@@ -216,11 +215,11 @@ let rebalance_preserves_bst (#a: Type) (cmp: cmp a) (t: wdm a)
   )
 
 //@AVL
-let rebalance_equal (#a: Type) (cmp: cmp a) (t: bst a cmp)
+let rebalance_avl_equal (#a: Type) (cmp: cmp a) (t: bst a cmp)
   : Lemma
-  (let new_t = rebalance_avl_wdm t in
-  rebalance_preserves_bst cmp t;
-  equal cmp t (rebalance_avl_wdm t))
+  (let new_t = rebalance_avl t in
+  rebalance_avl_preserves_bst cmp t;
+  equal cmp t (rebalance_avl t))
   =
   if Leaf? t then () else
   let Node data left right size height = t in
@@ -279,17 +278,18 @@ let rec insert_avl_aux (#a: Type)
       let new_left, b = insert_avl_aux r cmp left new_data in
       let new_t = merge_tree data new_left right in
       assert (is_wdm new_t);
-      let new_t2 = rebalance_avl_wdm new_t in
-      rebalance_avl_wds_size new_t;
+      let new_t2 = rebalance_avl new_t in
+      rebalance_avl_size new_t;
       new_t2, b
     end else begin
       let new_right, b = insert_avl_aux r cmp right new_data in
       let new_t = merge_tree data left new_right in
       assert (is_wdm new_t);
-      let new_t2 = rebalance_avl_wdm new_t in
-      rebalance_avl_wds_size new_t;
+      let new_t2 = rebalance_avl new_t in
+      rebalance_avl_size new_t;
       new_t2, b
     end
+#pop-options
 
 let rec skel_of_tree (#a: Type) (t: wdm a)
   : Pure (wdm nat)
@@ -305,16 +305,17 @@ let rec skel_of_tree (#a: Type) (t: wdm a)
       let new_right = skel_of_tree right in
       Node 0 new_left new_right size height
 
-let rec skel_balanced (#a: Type) (t: wdm a)
+let rec skel_balanced_local (#a: Type) (t: wdm a)
   : Lemma (
-  is_balanced t = is_balanced (skel_of_tree t)
+  is_balanced_local t = is_balanced_local (skel_of_tree t)
   )
   = match t with
   | Leaf -> ()
   | Node _ left right size height ->
-      skel_balanced left;
-      skel_balanced right
+      skel_balanced_local left;
+      skel_balanced_local right
 
+#push-options "--z3rlimit 25"
 let rec insert_in_place_preserves_skel (#a: Type)
   (r: bool) (cmp: cmp a) (t: avl a cmp) (new_data: a)
   : Lemma (
@@ -330,24 +331,26 @@ let rec insert_in_place_preserves_skel (#a: Type)
       insert_in_place_preserves_skel r cmp left new_data
     else
       insert_in_place_preserves_skel r cmp right new_data
+#pop-options
 
-let rebalance_balanced_id (#a: Type) (cmp: cmp a) (t: bst a cmp)
+let rebalance_avl_balanced_id (#a: Type) (cmp: cmp a) (t: bst a cmp)
   : Lemma
-  (requires is_balanced t)
-  (ensures rebalance_avl_wdm t == t)
+  (requires is_balanced_local t)
+  (ensures rebalance_avl t == t)
   = ()
 
 let not_balanced_is_not_null (#a: Type) (t: wdm a)
   : Lemma
-  (not (is_balanced t) ==> Node? t)
+  (not (is_balanced_local t) ==> Node? t)
   = ()
-let rebalance_height (#a: Type) (cmp: cmp a) (t: wdm a)
+
+let rebalance_avl_height (#a: Type) (cmp: cmp a) (t: wdm a)
   : Lemma
   (requires Node? t ==>
-    is_balanced (cleft t) /\
-    is_balanced (cright t))
+    is_balanced_local (cleft t) /\
+    is_balanced_local (cright t))
   (ensures
-    height_of_tree (rebalance_avl_wdm t) <= height_of_tree t)
+    height_of_tree (rebalance_avl t) <= height_of_tree t)
   =
   if Leaf? t then () else
   let Node data left right size height = t in
@@ -356,27 +359,28 @@ let rebalance_height (#a: Type) (cmp: cmp a) (t: wdm a)
     if hot_wdh lleft >= hot_wdh lright then (
       let r = rotate_right t in
       assert (Some? r);
-      rotate_right_h t
+      rotate_right_height t
     ) else (
       let r = rotate_left_right t in
       assert (Some? r);
-      rotate_left_right_h t
+      rotate_left_right_height t
     )
   ) else if hot_wdh right - hot_wdh left > 1 then (
     let Node rdata rleft rright rsize lright = right in
     if hot_wdh rleft > hot_wdh rright then (
       let r = rotate_right_left t in
       assert (Some? r);
-      rotate_right_left_h t
+      rotate_right_left_height t
     ) else (
       let r = rotate_left t in
       assert (Some? r);
-      rotate_left_h t
+      rotate_left_height t
     )
   ) else (
     ()
   )
 
+#push-options "--z3rlimit 25"
 let rec insert_avl_aux_bst (#a: Type)
   (r: bool) (cmp: cmp a) (t: avl a cmp) (new_data: a)
   : Lemma (
@@ -413,7 +417,7 @@ let rec insert_avl_aux_bst (#a: Type)
         let height_right = hot_wdh right in
         let new_height = M.max height_new_left height_right + 1 in
         let new_t = Node data new_left right new_size new_height in
-        let new_t2 = rebalance_avl_wdm new_t in
+        let new_t2 = rebalance_avl new_t in
         assert (new_t2 == rnew_t);
         assert (rb == b);
         // 2
@@ -430,13 +434,13 @@ let rec insert_avl_aux_bst (#a: Type)
             (key_left cmp data)
         end;
         assert (is_bst cmp new_t);
-        rebalance_preserves_bst cmp new_t;
+        rebalance_avl_preserves_bst cmp new_t;
         assert (is_bst cmp new_t2);
         // 3
         assert (
           (reveal b ==> add cmp t new_t new_data) /\
           (not (reveal b) ==> equal cmp t new_t));
-        rebalance_equal cmp new_t;
+        rebalance_avl_equal cmp new_t;
         assert (
           (reveal b ==> add cmp t new_t2 new_data) /\
           (not (reveal b) ==> equal cmp t new_t2));
@@ -450,7 +454,7 @@ let rec insert_avl_aux_bst (#a: Type)
         let height_new_right = hot_wdh new_right in
         let new_height = M.max height_left height_new_right + 1 in
         let new_t = Node data left new_right new_size new_height in
-        let new_t2 = rebalance_avl_wdm new_t in
+        let new_t2 = rebalance_avl new_t in
         assert (new_t2 == rnew_t);
         assert (rb == b);
         // 2
@@ -467,18 +471,19 @@ let rec insert_avl_aux_bst (#a: Type)
             (key_right cmp data)
         end;
         assert (is_bst cmp new_t);
-        rebalance_preserves_bst cmp new_t;
+        rebalance_avl_preserves_bst cmp new_t;
         assert (is_bst cmp new_t2);
         // 3
         assert (
           (reveal b ==> add cmp t new_t new_data) /\
           (not (reveal b) ==> equal cmp t new_t));
-        rebalance_equal cmp new_t;
+        rebalance_avl_equal cmp new_t;
         assert (
           (reveal b ==> add cmp t new_t2 new_data) /\
           (not (reveal b) ==> equal cmp t new_t2));
         ()
       end
+#pop-options
 
 #push-options "--z3rlimit 50"
 let rec insert_avl_aux_avl (#a: Type)
@@ -506,12 +511,12 @@ let rec insert_avl_aux_avl (#a: Type)
         assert (skel_of_tree rnew_t = skel_of_tree t);
         assert (hot_wdh rnew_t = hot_wdh t);
         // 2
-        assert (is_balanced (skel_of_tree rnew_t)
-              = is_balanced (skel_of_tree t));
-        skel_balanced t;
-        assert (is_balanced (skel_of_tree rnew_t));
-        skel_balanced rnew_t;
-        assert (is_balanced rnew_t);
+        assert (is_balanced_local (skel_of_tree rnew_t)
+              = is_balanced_local (skel_of_tree t));
+        skel_balanced_local t;
+        assert (is_balanced_local (skel_of_tree rnew_t));
+        skel_balanced_local rnew_t;
+        assert (is_balanced_local rnew_t);
         assert (is_avl cmp rnew_t)
       end else if delta < 0 then begin
         let new_left, b = insert_avl_aux r cmp left new_data in
@@ -522,14 +527,14 @@ let rec insert_avl_aux_avl (#a: Type)
         let height_right = hot_wdh right in
         let new_height = M.max height_new_left height_right + 1 in
         let new_t = Node data new_left right new_size new_height in
-        let new_t2 = rebalance_avl_wdm new_t in
+        let new_t2 = rebalance_avl new_t in
         assert (new_t2 == rnew_t);
         assert (rb == b);
         //assert (is_wdm t);
         // 2
         insert_avl_aux_bst r cmp t new_data;
         assert (is_bst cmp new_t2);
-        rebalance_preserves_bst cmp new_t;
+        rebalance_avl_preserves_bst cmp new_t;
         assert (is_bst cmp new_t);
         insert_avl_aux_avl r cmp left new_data;
         assert (is_avl cmp new_left);
@@ -537,7 +542,7 @@ let rec insert_avl_aux_avl (#a: Type)
         // TODO: new_left/right
         assert (hot_wdh t <= hot_wdh new_t);
         assert (hot_wdh new_t <= hot_wdh t + 1);
-        rebalance_avl_wds_proof cmp new_t data;
+        rebalance_avl_proof cmp new_t data;
         assert (is_avl cmp new_t2);
         // 1
         if not (reveal b) then begin
@@ -548,7 +553,7 @@ let rec insert_avl_aux_avl (#a: Type)
         end else begin
           assert (hot_wdh t <= hot_wdh new_t);
           assert (hot_wdh new_t <= hot_wdh t + 1);
-          rebalance_height cmp new_t;
+          rebalance_avl_height cmp new_t;
           assert (hot_wdh t <= hot_wdh new_t2);
           assert (hot_wdh new_t2 <= hot_wdh t + 1)
         end;
@@ -564,14 +569,14 @@ let rec insert_avl_aux_avl (#a: Type)
         let height_new_right = hot_wdh new_right in
         let new_height = M.max height_left height_new_right + 1 in
         let new_t = Node data left new_right new_size new_height in
-        let new_t2 = rebalance_avl_wdm new_t in
+        let new_t2 = rebalance_avl new_t in
         assert (new_t2 == rnew_t);
         assert (rb == b);
         //assert (is_wdm t);
         // 2
         insert_avl_aux_bst r cmp t new_data;
         assert (is_bst cmp new_t2);
-        rebalance_preserves_bst cmp new_t;
+        rebalance_avl_preserves_bst cmp new_t;
         assert (is_bst cmp new_t);
         insert_avl_aux_avl r cmp right new_data;
         assert (is_avl cmp left);
@@ -579,7 +584,7 @@ let rec insert_avl_aux_avl (#a: Type)
         // TODO: left/new_right
         assert (hot_wdh t <= hot_wdh new_t);
         assert (hot_wdh new_t <= hot_wdh t + 1);
-        rebalance_avl_wds_proof cmp new_t data;
+        rebalance_avl_proof cmp new_t data;
         assert (is_avl cmp new_t2);
         // 1
         if not (reveal b) then begin
@@ -590,7 +595,7 @@ let rec insert_avl_aux_avl (#a: Type)
         end else begin
           assert (hot_wdh t <= hot_wdh new_t);
           assert (hot_wdh new_t <= hot_wdh t + 1);
-          rebalance_height cmp new_t;
+          rebalance_avl_height cmp new_t;
           assert (hot_wdh t <= hot_wdh new_t2);
           assert (hot_wdh new_t2 <= hot_wdh t + 1)
         end;
@@ -645,18 +650,12 @@ let rec remove_leftmost_avl (#a: Type0)
     mem cmp t' leftmost = false /\
     //4 rest of the tree preserved
     add cmp t' t leftmost /\
-    //6 size decreased by 1
+    //5 size decreased by 1
     size_of_tree t' = size_of_tree t - 1 /\
-    //7
+    //6
     height_of_tree t - 1 <= height_of_tree t' /\
     height_of_tree t' <= height_of_tree t
   )
-    //(forall x. cmp x (snd r) <> 0
-    //  ==> mem cmp t x = mem cmp (fst r) x) /\
-    //5 subset
-    //subset cmp (fst r) t /\
-    //Node? (fst r) ==> is_balanced (cleft (fst r)) /\
-    //Node? (fst r) ==> is_balanced (cright (fst r)) /\
   =
   match t with
   | Node data Leaf right size _ ->
@@ -698,19 +697,19 @@ let rec remove_leftmost_avl (#a: Type0)
         (key_right cmp leftmost);
       // (3 : use 2)
       //smaller_not_mem cmp new_t leftmost;
-      let new_t2 = rebalance_avl_wdm new_t in
-      assert (is_balanced new_left);
-      assert (is_balanced right);
+      let new_t2 = rebalance_avl new_t in
+      assert (is_balanced_local new_left);
+      assert (is_balanced_local right);
       assert (height_of_tree left - 1 <= height_of_tree new_left);
       assert (height_of_tree new_left <= height_of_tree left);
       assert (height_of_tree right - height_of_tree new_left <= 2);
       assert (height_of_tree new_left - height_of_tree right <= 1);
-      rebalance_avl_wds_proof cmp new_t data;
+      rebalance_avl_proof cmp new_t data;
 
       // 1
       assert (mem cmp t leftmost = true);
       // 2
-      rebalance_equal cmp new_t;
+      rebalance_avl_equal cmp new_t;
       assert (subset cmp new_t2 new_t);
       subset_preserves_cond cmp
         new_t2 new_t (key_right cmp leftmost);
@@ -720,7 +719,7 @@ let rec remove_leftmost_avl (#a: Type0)
       // 5
       assert (add cmp new_t2 t leftmost);
       // 6
-      rebalance_avl_wds_size new_t;
+      rebalance_avl_size new_t;
       assert (size_of_tree new_t2 = size_of_tree t - 1);
       // 7
       assert (height_of_tree new_t2 <= height_of_tree t);
@@ -782,7 +781,7 @@ let delete_avl_aux0 (#a: Type0)
       let new_t = merge_tree succ_z l new_right in
       assert (sot_wds new_t = sz - 1);
       assert (hot_wdh new_t = new_height);
-      let new_t2 = rebalance_avl_wdm new_t in
+      let new_t2 = rebalance_avl new_t in
       // left: l <= z <= succ_z
       // z <= succ_z
       assert (forall_keys r (key_right cmp z));
@@ -823,14 +822,14 @@ let delete_avl_aux0 (#a: Type0)
       assert (add cmp new_t t data_to_rm);
       // new_t2
       // 1 a b
-      rebalance_preserves_bst cmp new_t;
-      rebalance_equal cmp new_t;
+      rebalance_avl_preserves_bst cmp new_t;
+      rebalance_avl_equal cmp new_t;
       assert (mem cmp t data_to_rm = true);
       assert (mem cmp new_t2 data_to_rm = false);
       // 2
       assert (add cmp new_t2 t data_to_rm);
       // 3
-      rebalance_avl_wds_size new_t;
+      rebalance_avl_size new_t;
       assert (size_of_tree new_t2 = size_of_tree t - 1);
       // 4: seemingly ok
       // avl
@@ -838,11 +837,12 @@ let delete_avl_aux0 (#a: Type0)
       assert (is_avl cmp new_right);
       assert (height_of_tree l - height_of_tree new_right <= 2);
       assert (height_of_tree new_right - height_of_tree l <= 2);
-      rebalance_avl_wds_proof cmp new_t succ_z;
+      rebalance_avl_proof cmp new_t succ_z;
       assert (is_avl cmp new_t2);
       new_t2
 #pop-options
 
+#push-options "--z3rlimit 25"
 let rec delete_avl_aux (#a: Type)
   (cmp:cmp a) (t: avl a cmp) (data_to_rm: a)
   : Pure (wdm a & erased bool)
@@ -862,18 +862,20 @@ let rec delete_avl_aux (#a: Type)
         let new_left, b = delete_avl_aux cmp left data_to_rm in
         let new_t = merge_tree data new_left right in
         assert (is_wdm new_t);
-        let new_t2 = rebalance_avl_wdm new_t in
-        rebalance_avl_wds_size new_t;
+        let new_t2 = rebalance_avl new_t in
+        rebalance_avl_size new_t;
         new_t2, b
       end else begin
         let new_right, b = delete_avl_aux cmp right data_to_rm in
         let new_t = merge_tree data left new_right in
         assert (is_wdm new_t);
-        let new_t2 = rebalance_avl_wdm new_t in
-        rebalance_avl_wds_size new_t;
+        let new_t2 = rebalance_avl new_t in
+        rebalance_avl_size new_t;
         new_t2, b
       end
+#pop-options
 
+#push-options "--z3rlimit 25"
 let rec delete_avl_aux_bst (#a: Type0)
   (cmp:cmp a) (t: avl a cmp) (data_to_rm: a)
   : Lemma (
@@ -904,7 +906,7 @@ let rec delete_avl_aux_bst (#a: Type0)
         let height_right = hot_wdh right in
         let new_height = M.max height_new_left height_right + 1 in
         let new_t = Node data new_left right new_size new_height in
-        let new_t2 = rebalance_avl_wdm new_t in
+        let new_t2 = rebalance_avl new_t in
         assert (new_t2 == rnew_t);
         assert (rb == b);
 
@@ -916,7 +918,7 @@ let rec delete_avl_aux_bst (#a: Type0)
         assert (forall_keys new_left (key_left cmp data));
         assert (forall_keys right (key_right cmp data));
         assert (is_bst cmp new_t);
-        rebalance_preserves_bst cmp new_t;
+        rebalance_avl_preserves_bst cmp new_t;
         assert (is_bst cmp new_t2);
 
         assert (mem cmp new_left data_to_rm = false);
@@ -925,7 +927,7 @@ let rec delete_avl_aux_bst (#a: Type0)
           (key_right cmp data_to_rm);
         smaller_not_mem cmp right data_to_rm;
         assert (mem cmp new_t data_to_rm = false);
-        rebalance_equal cmp new_t;
+        rebalance_avl_equal cmp new_t;
         assert (mem cmp new_t2 data_to_rm = false);
         assert (
          (reveal b ==> add cmp new_t t data_to_rm) /\
@@ -944,7 +946,7 @@ let rec delete_avl_aux_bst (#a: Type0)
         let height_new_right = hot_wdh new_right in
         let new_height = M.max height_left height_new_right + 1 in
         let new_t = Node data left new_right new_size new_height in
-        let new_t2 = rebalance_avl_wdm new_t in
+        let new_t2 = rebalance_avl new_t in
         assert (new_t2 == rnew_t);
         assert (rb == b);
 
@@ -957,7 +959,7 @@ let rec delete_avl_aux_bst (#a: Type0)
         assert (forall_keys new_right (key_right cmp data));
         assert (forall_keys left (key_left cmp data));
         assert (is_bst cmp new_t);
-        rebalance_preserves_bst cmp new_t;
+        rebalance_avl_preserves_bst cmp new_t;
         assert (is_bst cmp new_t2);
 
         assert (mem cmp new_right data_to_rm = false);
@@ -966,7 +968,7 @@ let rec delete_avl_aux_bst (#a: Type0)
           (key_left cmp data_to_rm);
         greater_not_mem cmp left data_to_rm;
         assert (mem cmp new_t data_to_rm = false);
-        rebalance_equal cmp new_t;
+        rebalance_avl_equal cmp new_t;
         assert (mem cmp new_t2 data_to_rm = false);
         assert (
          (reveal b ==> add cmp new_t t data_to_rm) /\
@@ -976,6 +978,7 @@ let rec delete_avl_aux_bst (#a: Type0)
          (not (reveal b) ==> equal cmp new_t2 t));
         ()
       end
+#pop-options
 
 #push-options "--z3rlimit 50"
 let rec delete_avl_aux_avl (#a: Type0)
@@ -1005,22 +1008,22 @@ let rec delete_avl_aux_avl (#a: Type0)
         let height_right = hot_wdh right in
         let new_height = M.max height_new_left height_right + 1 in
         let new_t = Node data new_left right new_size new_height in
-        let new_t2 = rebalance_avl_wdm new_t in
+        let new_t2 = rebalance_avl new_t in
         assert (new_t2 == rnew_t);
         assert (rb == b);
 
         delete_avl_aux_bst cmp t data_to_rm;
         assert (is_bst cmp new_t2);
-        rebalance_preserves_bst cmp new_t;
+        rebalance_avl_preserves_bst cmp new_t;
         assert (is_bst cmp new_t);
         delete_avl_aux_avl cmp left data_to_rm;
         assert (is_avl cmp new_left);
         assert (is_avl cmp right);
         assert (hot_wdh new_left - hot_wdh right <= 2);
         assert (hot_wdh right - hot_wdh new_left <= 2);
-        rebalance_avl_wds_proof cmp new_t data;
+        rebalance_avl_proof cmp new_t data;
         assert (is_avl cmp new_t2);
-        rebalance_height cmp new_t;
+        rebalance_avl_height cmp new_t;
         ()
 
       end else begin
@@ -1032,22 +1035,22 @@ let rec delete_avl_aux_avl (#a: Type0)
         let height_new_right = hot_wdh new_right in
         let new_height = M.max height_left height_new_right + 1 in
         let new_t = Node data left new_right new_size new_height in
-        let new_t2 = rebalance_avl_wdm new_t in
+        let new_t2 = rebalance_avl new_t in
         assert (new_t2 == rnew_t);
         assert (rb == b);
 
         delete_avl_aux_bst cmp t data_to_rm;
         assert (is_bst cmp new_t2);
-        rebalance_preserves_bst cmp new_t;
+        rebalance_avl_preserves_bst cmp new_t;
         assert (is_bst cmp new_t);
         delete_avl_aux_avl cmp right data_to_rm;
         assert (is_avl cmp new_right);
         assert (is_avl cmp left);
         assert (hot_wdh new_right - hot_wdh left <= 2);
         assert (hot_wdh left - hot_wdh new_right <= 2);
-        rebalance_avl_wds_proof cmp new_t data;
+        rebalance_avl_proof cmp new_t data;
         assert (is_avl cmp new_t2);
-        rebalance_height cmp new_t;
+        rebalance_avl_height cmp new_t;
         ()
       end
 #pop-options
